tests/lean/run/induction_generalizing_bug.lean
@@ -1,0 +1,8 @@
+open nat
+
+example (n : nat) (h : n > 0) : succ n > 0 ∧ n = n :=
+begin
+  split,
+  induction n generalizing h,
+  all_goals { admit },
+end
